progress on Compiler

theories/LAM/Compiler.v
@@ -6,209 +6,23 @@ Require Import Vector List.
 Require Import Undecidability.TM.Util.TM_facts.
 
 From Undecidability Require Import ProgrammingTools LM_heap_def WriteValue Copy.
-From Undecidability.LAM Require Import TM.Alphabets TM.StepTM TM.HaltingProblem.
+From Undecidability.L.AbstractMachines.TM_LHeapInterpreter Require Import Alphabets StepTM M_LHeapInterpreter.
 From Undecidability Require Import TM.TM L.AbstractMachines.FlatPro.LM_heap_correct.
 
 From Undecidability Require Import L.L TM.TM.
 Require Import List.
 Import ListNotations.
 
-Definition encTM {Σ : Type} (s b : Σ) (l : list bool) := @midtape Σ [] b (fold_right (fun (x : bool) r => (if x then s else b) :: r) nil l).
 
 Import VectorNotations.
 
-Definition TM_computable {k} (R : Vector.t (list bool) k -> (list bool) -> Prop) := 
-  exists n : nat, exists Σ : finType, exists s b : Σ, s <> b /\ 
-  exists M : TM Σ (k + 1 + n),
-  forall v : Vector.t (list bool) k, 
-  (forall m, R v m <-> exists q t, TM.eval M (start M) ((Vector.map (encTM s b) v ++ [niltape]) ++ Vector.const niltape n) q t
-                                /\ nth_error (Vector.to_list t) k = Some (encTM s b m)) /\
-  (forall q t, TM.eval M (start M) ((Vector.map (encTM s b) v ++ [niltape]) ++ Vector.const niltape n) q t ->
-          exists m, nth_error (Vector.to_list t) k = Some (encTM s b m)).
-
-
-Definition TM_computable_rel {k} (R : Vector.t (list bool) k -> (list bool) -> Prop) := 
-  exists n : nat, exists Σ : finType, exists s b : Σ, s <> b /\ 
-  exists M : pTM Σ unit (k + 1 + n),
-    Realise M (fun t '(_, t') =>
-                                       forall v, t = (Vector.map (encTM s b) v ++ [niltape]) ++ Vector.const niltape n ->
-                                            exists m, nth_error (Vector.to_list t') k = Some (encTM s b m) /\ R v m) /\
-    exists f,
-      TerminatesIn (projT1 M) (fun t i => exists v m, R v m /\ t = (Vector.map (encTM s b) v ++ [niltape]) ++ Vector.const niltape n /\ i >= f k v).
+From Undecidability.LAM Require Import Compiler_spec Compiler_facts.
 
 Require Import Equations.Prop.DepElim.
 
-Lemma nth_error_to_list {X n} (v : Vector.t X n) i k :
-  k = (proj1_sig (Fin.to_nat i)) ->
-  nth_error (Vector.to_list v) k = Some (Vector.nth v i).
-Proof.
-  intros ->. induction v; cbn.
-  - inversion i.
-  - dependent destruct i; cbn.
-    + reflexivity.
-    + destruct (Fin.to_nat p) as (i, P) eqn:E. cbn.
-      fold (to_list v).
-      specialize (IHv (Fin.of_nat_lt P)). cbn in *.
-      rewrite Fin.to_nat_of_nat in IHv. cbn in IHv.
-      now rewrite <- (Fin.of_nat_to_nat_inv p), E. 
-Qed.
-
-Lemma encTM_inj {Σ} (sym_s sym_b : Σ) n1 n2 :
-  sym_s <> sym_b -> encTM sym_s sym_b n1 = encTM sym_s sym_b n2 -> n1 = n2.
-Proof.
-  intros Hdiff.
-  induction n1 in n2 |- *.
-  - destruct n2; now inversion 1.
-  - destruct n2; inversion 1.
-    destruct a, b.
-    + f_equal. eapply IHn1. unfold encTM. congruence.
-    + now exfalso.
-    + now exfalso.
-    + f_equal. eapply IHn1. unfold encTM. congruence.
-Qed.
-
-Lemma TM_computable_rel_spec k R :
-  functional R ->
-  @TM_computable_rel k R -> @TM_computable k R.
-Proof.
-  intros Hfun (n & Σ & s & b & Hdiff & [M lab] & H1 & f & H2).
-  exists n, Σ, s, b. split. exact Hdiff. exists M.
-  intros v. split.
-  - intros m. split.
-    + intros HR.
-      destruct (H2 ((Vector.map (encTM s b) v ++ [niltape]) ++ Vector.const niltape n) (f k v)) as [[q' t'] Hconf].
-      * exists v, m. split. eauto. split. reflexivity. lia.
-      * exists q', t'. split. eapply TM_eval_iff. eexists. eapply Hconf.
-        eapply H1 in Hconf as (m' & Hm1 & Hm2). reflexivity.
-        now pose proof (Hfun _ _ _ HR Hm2) as ->.
-    + intros (q' & t' & [steps Hter] % TM_eval_iff & Hout).
-      eapply H1 in Hter as (m' & Hm1 & Hm2). reflexivity.
-      cbn -[to_list] in *. 
-      rewrite Hm1 in Hout.
-      enough (m = m') by now subst.
-      eapply encTM_inj; eauto. congruence.
-  - intros q t [steps Hter] % TM_eval_iff.
-    eapply H1 in Hter as (m & Hm1 & Hm2). reflexivity.
-    exists m. eassumption.
-Qed.
-
-Definition TM_computable_rel' {k} (R : Vector.t (list bool) k -> (list bool) -> Prop) := 
-  exists n : nat, exists Σ : finType, exists s b : Σ, s <> b /\ 
-  exists M : pTM Σ unit (1 + n + k),
-    Realise M (fun t '(_, t') =>
-                                       forall v, t = ([niltape] ++ Vector.const niltape n ++ (Vector.map (encTM s b) v)) ->
-                                            exists m, Vector.hd t' = encTM s b m /\ R v m) /\
-    exists f,
-      TerminatesIn (projT1 M) (fun t i => exists v m, R v m /\ t = ([niltape] ++ Vector.const niltape n ++ (Vector.map (encTM s b) v)) /\ i >= f k v).
-
-Lemma Vector_nth_L {X k1 k2} (v1 : Vector.t X k1) (v2 : Vector.t X k2) i :
-  (v1 ++ v2)[@ Fin.L k2 i] = v1[@i].
-Proof.
-  revert k2 v2 i.
-  dependent induction v1; intros.
-  - dependent destruct i.
-  - dependent destruct i.
-    + reflexivity.
-    + cbn. eapply IHv1.
-Qed.
-
-Lemma Vector_nth_R {X k1 k2} (v1 : Vector.t X k1) (v2 : Vector.t X k2) i :
-  (v1 ++ v2)[@ Fin.R k1 i] = v2[@i].
-Proof.
-  revert k2 v2 i.
-  dependent induction v1; intros.
-  - reflexivity.
-  - cbn. eapply IHv1.
-Qed.
-
-Lemma Vector_map_app {X Y k1 k2} (v1 : Vector.t X k1) (v2 : Vector.t X k2) (f : X -> Y) :
-  Vector.map f (v1 ++ v2) = Vector.map f v1 ++ Vector.map f v2.
-Proof.
-  induction v1; cbn; congruence.
-Qed.
-
-Lemma TM_computable_rel'_spec k R :
-  functional R ->
-  @TM_computable_rel' k R -> TM_computable R.
-Proof.
-  intros Hfun (n & Σ & s & b & Hdiff & M & H1 & f & H2).
-  eapply TM_computable_rel_spec. eassumption.
-  exists n, Σ, s, b. split. exact Hdiff.
-  eexists (LiftTapes M (Fin.L n (Fin.R k Fin0) :::  tabulate (n := n) (fun x => Fin.R (k + 1) x) ++ (tabulate (n := k) (fun x => Fin.L n (Fin.L 1 x))))).
-  split.
-  - eapply Realise_monotone. eapply LiftTapes_Realise. admit. eapply H1.
-    intros tps [[] tps'] H v ->.
-    cbn in H. destruct H as [H H'].
-    destruct (H v) as (m & Hm1 & Hm2).
-    + f_equal.
-      * rewrite Vector_nth_L, Vector_nth_R. reflexivity.
-      * admit.
-    + exists m. split. 2:eassumption. erewrite nth_error_to_list, Hm1. reflexivity.
-      rewrite Fin.L_sanity, Fin.R_sanity. cbn. lia.
-  - exists f. eapply TerminatesIn_monotone.
-    eapply LiftTapes_Terminates. admit. eapply H2.
-    intros tps i (v & m & HR & -> & Hf); subst.
-    exists v, m. split. eauto. split; try eassumption.
-    { unfold select. clear. cbn. f_equal.
-      now rewrite Vector_nth_L, Vector_nth_R.
-      rewrite Vector_map_app. f_equal.
-      - admit.
-      - admit.
-    }
-Admitted.
-
-Definition encL (l : list bool) := list_enc l.
-
-Definition L_computable {k} (R : Vector.t (list bool) k -> (list bool) -> Prop) := 
-  exists s, forall v : Vector.t (list bool) k, 
-      (forall m, R v m <-> L.eval (Vector.fold_left (fun s n => L.app s (encL n)) s v) (encL m)) /\
-      (forall o, L.eval (Vector.fold_left (fun s n => L.app s (encL n)) s v) o -> exists m, o = encL m).
-
-Fixpoint encL' (l : list bool) :=
-  match l with
-  | nil => enc (@List.nil bool)
-  | b :: l => L.app (L.app (ext (@List.cons bool)) (ext b)) (encL' l)
-  end%list.
-
-Definition L_computable' {k} (R : Vector.t (list bool) k -> (list bool) -> Prop) := 
-  exists s, forall v : Vector.t (list bool) k, 
-      (forall m, R v m <-> L.eval (Vector.fold_left (fun s n => L.app s (encL' n)) s v) (encL m)) /\
-      (forall o, L.eval (Vector.fold_left (fun s n => L.app s (encL' n)) s v) o -> exists m, o = encL m).
-
-Lemma encL_encL' l :
-  encL' l >* encL l.
-Proof.
-  induction l.
-  - reflexivity.
-  - cbn. Lsimpl.
-Admitted.
-
-Lemma encL_encL'_fold_eval s t {k} (v : Vector.t (list bool) k) res :
-  s >* t ->
-  L.eval (Vector.fold_left (fun (s0 : term) (n : list bool) => L.app s0 (encL' n)) s v) res <->
-  L.eval (Vector.fold_left (fun (s0 : term) (n : list bool) => L.app s0 (encL n)) t v) res.
-Proof.
-  intros Hst.
-  induction v as [ | l k v IH] in s, t, Hst |- *; cbn.
-  - rewrite !eval_iff. split; intros []; split; eauto.
-    + eapply equiv_lambda. eauto. now rewrite <- Hst, H.
-    + now rewrite Hst.
-  - rewrite IH. reflexivity.
-    now rewrite encL_encL', Hst.
-Qed.
-
-Lemma L_computable'_spec k R :
-  @L_computable k R -> L_computable' R.
-Proof.
-  intros [s H]. exists s. intros v.
-  specialize (H v) as [H1 H2].
-  split.
-  - intros res. now rewrite H1, encL_encL'_fold_eval.
-  - intros res H. eapply encL_encL'_fold_eval in H. 2:reflexivity.
-    now eapply H2 in H.
-Qed.
-
 Import VectorNotations.
+
+Set Default Proof Using "Type".
 
 Section APP_right.
 
@@ -216,7 +30,11 @@ Section APP_right.
   Admitted.
 
   Lemma APP_right_realise :
-    Realise APP_right (fun t '(r, t') => forall s1 s2 : L.term, t[@Fin0] ≃ compile s1 -> t[@Fin1] ≃ compile s2 -> t'[@Fin0] ≃ compile (L.app s1 s2)).
+    Realise APP_right (fun t '(r, t') =>
+    forall s1 s2 : L.term,
+    t[@Fin0] ≃ compile s1
+    -> t[@Fin1] ≃ compile s2
+    -> t'[@Fin0] ≃ compile (L.app s1 s2)).
   Admitted.
 
 End APP_right.
@@ -232,11 +50,10 @@ Section mk_init_one.
 
   Lemma M_init_one_realise :
     Realise M_init_one (fun t '(r, t') =>
-                          forall n,
+                          forall (n:list bool) (ter : L.term),
                             t[@Fin0] = encTM s b n ->
                             (* isRight (t[@Fin1]) -> *)
                             (* isRight (t[@Fin2]) -> *)
-                          forall ter : L.term,
                             t[@Fin1] ≃ compile ter ->
                             t'[@Fin1] ≃ compile (L.app ter (encL' n))
                        ).
@@ -262,7 +79,7 @@ Section mk_init.
   Variable sim : term.
 
   Definition M_init k : pTM (Σ) ^+ unit (n + k). 
-  Proof.
+  Proof using All.
   (*   induction k as [ | k_ M_init]. *)
   (*   - exact (LiftTapes (WriteValue (encode (compile sim))) [| Fin.R ( k + 1) (help1) |]). *)
   (*   - refine ( *)
@@ -274,7 +91,7 @@ Section mk_init.
 
   Theorem M_init_rel k :
     Realise (M_init k) (fun t '(r, t') =>
-                 forall v, 
+                 forall (v:Vector.t (list bool) k), 
                    t = Vector.const niltape n ++ Vector.map (encTM s b) v ->
                    t'[@Fin.L k output1] ≃ [(0, compile (Vector.fold_left (fun s l_i => L.app s (encL l_i)) sim v))]%list /\
                    t'[@Fin.L k output2] ≃ []%list /\
@@ -321,37 +138,29 @@ Section conv_output.
 
   Variable Σ : finType.
   Variable s b : Σ^+.
-  Context {Henc1 : codable Σ Heap}.
-  Context {Henc2 : codable Σ (list HClos)}.
   Context {Henc3 : codable Σ (list Tok)}.
     
-  Variable n : nat.
 
-  Variable i_l : Fin.t n.
-  Variable o_m : Fin.t n.
-
-  Definition M_out : pTM (Σ) ^+ unit n. Admitted.
+  Definition M_out : pTM (Σ) ^+ unit 2. Admitted.
 
   Theorem M_out_realise :
     Realise M_out (fun t '(r, t') =>
-                     forall l : list bool, t[@i_l] ≃ compile (list_enc l) ->
-                                   t'[@o_m] = encTM s b l).
+                     forall l : list bool, t[@Fin0] ≃ compile (list_enc l) ->
+                        t[@Fin1] = niltape ->
+                        t'[@Fin1] = encTM s b l).
   Admitted.
 
 End conv_output.
 
 Section MK_isRight.
 
-  Variable n : nat.
   Context {Σ : finType}.
-  Variable s : Σ.
-  Variable i : Fin.t n.
 
-  Definition MK_isRight : pTM Σ unit n.
+  Definition MK_isRight : pTM Σ unit 1.
   Admitted.
 
   Lemma MK_isRight_realise :
-    Realise MK_isRight (fun t '(r, t') => isRight (t'[@i]) /\ forall j, not_index [| i |] j -> t'[@j] = t[@j]).
+    Realise MK_isRight (fun t '(r, t') => isRight (t'[@Fin0])).
   Admitted.
 
 End MK_isRight.
@@ -396,20 +205,20 @@ Section main.
   Definition garb : Σ := inl UNKNOWN.
 
   Definition M_main : pTM Σ unit (1 + n_main + k).
-  Proof.
+  Proof using k s.
     refine (
         M_init sym_s sym_b Fin1 Fin2 Fin3 Fin4 Fin5 s k ;;
-        MK_isRight garb ( aux Fin5 ) ;;
-        MK_isRight garb ( aux Fin6 ) ;;
-        MK_isRight garb ( aux Fin7 ) ;;
-        MK_isRight garb ( aux Fin8 ) ;;
-        MK_isRight garb ( aux Fin9 ) ;;
-        MK_isRight garb ( aux Fin10) ;;
-        MK_isRight garb ( aux Fin11) ;;
-        MK_isRight garb ( aux Fin12) ;;
+        LiftTapes MK_isRight [|aux Fin5 |] ;;
+        LiftTapes MK_isRight [|aux Fin6 |] ;;
+        LiftTapes MK_isRight [|aux Fin7 |] ;;
+        LiftTapes MK_isRight [|aux Fin8 |] ;;
+        LiftTapes MK_isRight [|aux Fin9 |] ;;
+        LiftTapes MK_isRight [|aux Fin10 |] ;;
+        LiftTapes MK_isRight [|aux Fin11 |] ;;
+        LiftTapes MK_isRight [|aux Fin12 |] ;;
         LiftAlphabet (LiftTapes Loop [| aux Fin0 ; aux Fin1 ; aux Fin2 ; aux Fin5 ; aux Fin6 ; aux Fin7 ; aux Fin8 ; aux Fin9 ; aux Fin10 ; aux Fin11 ; aux Fin12 |]) _ (inl UNKNOWN)  ;;
-        M_unf (aux Fin1) (aux Fin2) (aux Fin13) ;;
-        M_out sym_s sym_b (aux Fin13) Fin0
+        M_unf (aux Fin1) (aux Fin2) (aux Fin13);;
+        (LiftTapes (M_out sym_s sym_b) [|(aux Fin13);Fin0|])
       ).
     all: exact todo.
   Defined.
@@ -425,18 +234,9 @@ Section main.
   Proof.
     eapply Realise_monotone.
     {
-      eapply Seq_Realise. eapply M_init_rel.
-      eapply Seq_Realise. eapply MK_isRight_realise.
-      eapply Seq_Realise. eapply MK_isRight_realise.
-      eapply Seq_Realise. eapply MK_isRight_realise.
-      eapply Seq_Realise. eapply MK_isRight_realise.
-      eapply Seq_Realise. eapply MK_isRight_realise.
-      eapply Seq_Realise. eapply MK_isRight_realise.
-      eapply Seq_Realise. eapply MK_isRight_realise.
-      eapply Seq_Realise. eapply MK_isRight_realise.
-      eapply Seq_Realise. eapply LiftAlphabet_Realise. eapply LiftTapes_Realise. admit. eapply Loop_Realise.
-      eapply Seq_Realise. eapply M_unf_realise.
-      eapply M_out_realise.
+      unfold M_main.
+      TM_Correct.
+      all:eauto using M_init_rel, MK_isRight_realise, Loop_Realise, M_unf_realise, M_out_realise.
     }
     (* intros tin ([] & tout) H v ->. *)
     (* unfold n_main in *. cbn in tout. *)
@@ -485,7 +285,7 @@ Proof.
   eapply L_computable_function; eauto.
   eapply L_computable'_spec in H as [sim Hsim].
   exists n_main, Σ, sym_s, sym_b. split. eapply syms_diff. exists (M_main k sim). split.
-  - eapply Realise_monotone. { eapply M_main_realise. eapply Hsim. intros. now eapply Hsim. }
+  - eapply Realise_monotone. { eapply M_main_realise. }
     intros t [[] t'] H v ->.
     destruct (H v) as [m [Hm1 Hm2]]. reflexivity.
     exists m. split; eauto. rewrite <- Hm1.
