theories/LAM/encTM_boolList.v
@@ -1,0 +1,88 @@
+Require Import PslBase.FiniteTypes.FinTypes PslBase.Vectors.Vectors.
+Require Import Undecidability.TM.Util.TM_facts.
+From Undecidability Require Import ProgrammingTools WriteValue Copy.
+
+Require Import PslBase.FiniteTypes.FinTypes PslBase.Vectors.Vectors.
+Require Import Vector List.
+
+From Undecidability.TM.Compound Require Import MoveToSymbol.
+From Undecidability.TM.Code Require Import CaseBool CaseList Copy.
+
+From Undecidability.LAM Require Import Compiler_spec.
+
+Import ListNotations.
+Import VectorNotations.
+
+
+Module boolList2encTM.
+Section Fix.
+
+  Variable Σ : finType.
+  Variable s b : Σ^+.
+
+  Variable (retr_list : Retract (sigList bool) Σ).
+  Local Instance retr_bool : Retract bool Σ := ComposeRetract retr_list (Retract_sigList_X _).
+
+  Definition M__step : pTM (Σ) ^+ (option unit) 3 := 
+    If (LiftTapes (ChangeAlphabet (CaseList _) retr_list) [|Fin0;Fin2|])
+       (Switch (LiftTapes (ChangeAlphabet (CaseBool) retr_bool) [|Fin2|])
+            (fun x =>
+            LiftTapes (WriteMove (if x then s else b) Lmove) [|Fin1|];;
+            Return Nop None))
+       (Reset _ @[|Fin0|];;Return (LiftTapes (Write b) [|Fin1|]) (Some tt)).
+  
+  Definition M__loop := While M__step.
+  
+  Definition Realises__loop :
+    Realise M__loop (fun t '(r, t') =>
+      forall (l l': list bool),
+        t[@Fin0] ≃ l ->
+        right t[@Fin1] = map (fun (x:bool) => if x then s else b) l' ->
+        length (left t[@Fin1]) <= length l ->
+        isRight (t[@Fin2]) ->
+        t'[@Fin1] = encTM s b (rev l++l')
+        /\ (isRight (t'[@Fin0]) /\ isRight (t'[@Fin2]))).
+  Proof.
+    eapply Realise_monotone.
+    {unfold M__loop,M__step.  TM_Correct_noSwitchAuto. TM_Correct. cbn. intros. TM_Correct. 
+      eapply Reset_Realise with (X:=list bool).
+    }
+    eapply WhileInduction; intros;hnf.
+    - destruct HLastStep;TMSimp.
+      specialize (H3 l). modpon H3. 
+      destruct l. 2:contradiction H3.
+      TMSimp;cbn in *. simpl_surject.
+      modpon H4. split. 2:easy.
+      rewrite H0. unfold encTM. 
+      destruct tin1 as [ | | | ] eqn:Heq;cbn in *. 
+      all:(destruct l';revert Heq;inv H0;cbn;intros Heq).  
+      1,2:reflexivity.
+      1:exfalso;nia. 
+      all: destruct l;[reflexivity | ].
+      all:exfalso; revert H1; clear;cbn. all:nia.
+    - destruct HStar. all:TMSimp. simpl_surject.
+      modpon H3. destruct l. contradiction.
+      TMSimp. simpl_surject.
+      modpon H4. TMSimp.
+      autorewrite with tape in HLastStep.
+      rewrite H0 in HLastStep. rewrite tl_length in HLastStep.
+      specialize (HLastStep l (cons b0 l')).
+      modpon  HLastStep. lia.
+      split. 2:easy. autorewrite with list. assumption.
+  Qed.
+
+  Definition M : pTM (Σ) ^+ unit 3 :=
+    LiftTapes (MoveToSymbol (fun _ => false) id) [|Fin1|];;M__loop.
+
+  Theorem Realises :
+    Realise M (fun t '(r, t') =>
+                     forall (l : list bool),
+                        t[@Fin0] ≃ l ->
+                        sizeOfTape(t[@Fin1]) <= length l + 1 ->
+                        isRight (t[@Fin2]) ->
+                        t'[@Fin1] = encTM s b (rev l)
+                        /\ (isRight (t'[@Fin1]) /\ isRight (t'[@Fin2]))).
+  Proof.    
+  Admitted.
+End Fix.
+End boolList2encTM.
