theories/TM/Code/CaseBool.v
@@ -1,0 +1,53 @@
+(** * Constructors and Deconstructors for Bool *)
+
+From Undecidability Require Import ProgrammingTools Code.
+
+Section CaseBool.
+
+  Local Notation sig := bool.
+ 
+  Definition CaseBool : pTM bool^+ bool 1 :=
+    Move Rmove;;
+    Switch (ReadChar)
+    (fun s => match s with
+           | Some (inr x) => Return (Move Rmove) x
+           | _ => Return (Nop) default
+           end).
+
+  Definition CaseBool_Rel : pRel bool^+ bool 1 :=
+    fun tin '(yout, tout) => forall (x : sig) (s : nat), tin[@Fin0] ≃(;s) x -> isRight_size tout[@Fin0] (S(S(s))) /\ yout = x.
+
+  Definition CaseBool_steps := 5.
+
+
+
+  Lemma CaseBool_Sem : CaseBool ⊨c(CaseBool_steps) CaseBool_Rel.
+  Proof.
+    TM_Correct_noSwitchAuto.
+    unfold CaseBool_steps. eapply RealiseIn_monotone.
+    { unfold CaseBool. TM_Correct. intros b.
+      destructBoth b as [ [] | ].
+      all:eapply RealiseIn_monotone';[TM_Correct | ]. 2:reflexivity. all:Lia.nia. }
+    { Lia.nia. }
+    {
+      intros tin (yout, tout) H. intros x s HEncX.
+      destruct HEncX as (ls&HEncX&Hs).  
+      TMSimp. split. 2:auto. hnf. do 2 eexists. split;[f_equal| ]. cbn;nia.
+    }
+  Qed.
+
+  (** There is no need for a constructor, just use [WriteValue] *)
+
+End CaseBool.
+
+
+Arguments CaseBool : simpl never.
+
+Ltac smpl_TM_CaseBool :=
+  lazymatch goal with
+  | [ |- CaseBool ⊨ _ ] => eapply RealiseIn_Realise; apply CaseBool_Sem
+  | [ |- CaseBool ⊨c(_) _ ] => apply CaseBool_Sem
+  | [ |- projT1 CaseBool ↓ _ ] => eapply RealiseIn_TerminatesIn; apply CaseBool_Sem
+  end.
+
+Smpl Add smpl_TM_CaseBool : TM_Correct.
